veristar/clause_universe.v
@@ -1,3 +1,4 @@
+Load loadpath.
 Require MSets.
 Require Coq.Structures.Orders.
 Require Coq.Structures.OrdersFacts.
