veristar/extract/loadpath.v
@@ -1,0 +1,10 @@
+Add LoadPath "../../compositional_compcert".
+Add LoadPath "../../compcert/lib".
+Add LoadPath "../../compcert/flocq/Appli".
+Add LoadPath "../../compcert/flocq/Calc".
+Add LoadPath "../../compcert/flocq/Core".
+Add LoadPath "../../compcert/flocq/Prop".
+Add LoadPath "../../compcert/common".
+Add LoadPath "../../compcert/cfrontend".
+Add LoadPath "../..". 
+Add LoadPath "../../..".
